Core/SingConds.v
@@ -1,0 +1,124 @@
+From LHL.Core Require Import
+  LogicFacts
+  Traces
+  Specs
+  Logic.
+
+Definition SPrec {T E F} (VE : Spec T E) (VF : Spec T F) :=
+  InterState F VE ->
+  Poss VF ->
+  Prop.
+
+Definition SRelt {T E F} (VE : Spec T E) (VF : Spec T F) :=
+  InterState F VE ->
+  Poss VF ->
+  InterState F VE ->
+  Poss VF ->
+  Prop.
+
+Definition LiftSPrec {T E F} {VE : Spec T E} {VF : Spec T F} (P : SPrec VE VF) : Prec VE VF :=
+  fun s xs =>
+    exists x, xs = eq x /\
+      P s x.
+Coercion LiftSPrec : SPrec >-> Prec.
+
+Definition LiftSRelt {T E F} {VE : Spec T E} {VF : Spec T F} (R : SRelt VE VF) : Relt VE VF :=
+  fun s xs t ys =>
+    forall x, xs = eq x ->
+      exists y, ys = eq y /\
+        R s x t y.
+Coercion LiftSRelt : SRelt >-> Relt.
+
+Definition SPrecCompose {T E F} {VE : Spec T E} {VF : Spec T F} (P : SPrec VE VF) (R : SRelt VE VF) : SPrec VE VF :=
+  fun t σ => exists s ρ, P s ρ /\ R s ρ t σ.
+
+Notation "R <<S G" := (SPrecCompose R G) (left associativity, at level 37).
+
+Definition SReltCompose {T E F} {VE : Spec T E} {VF : Spec T F} (R G : SRelt VE VF) : SRelt VE VF :=
+  fun s ρ r τ => exists t σ, R s ρ t σ /\ G t σ r τ.
+Notation "R S>> G" := (SReltCompose R G) (right associativity, at level 39).
+
+Class HasSSub A :=
+  ssub : A -> A -> Prop.
+Notation "P S=> Q" := (ssub P Q) (right associativity, at level 41).
+
+Global Instance subSPrec {T E F} {VE : Spec T E} {VF : Spec T F} : HasSSub (SPrec VE VF) :=
+  fun P Q => forall s ρ, P s ρ -> Q s ρ.
+
+Global Instance subSRelt {T E F} {VE : Spec T E} {VF : Spec T F} : HasSSub (SRelt VE VF) :=
+  fun P Q => forall s ρ t σ, P s ρ t σ -> Q s ρ t σ.
+
+Class HasSStable {T E F} {VE : Spec T E} {VF : Spec T F} A :=
+  SStable : SRelt VE VF -> A -> Prop.
+
+Global Instance stableSRelt {T E F} {VE : Spec T E} {VF : Spec T F} : HasSStable (SRelt VE VF) :=
+  fun R Q => (Q S>> R S=> Q).
+
+Global Instance stableSPrec {T E F} {VE : Spec T E} {VF : Spec T F} : HasSStable (SPrec VE VF) :=
+  fun R P => P <<S R S=> P.
+
+Lemma liftSPrecStable {T E F} {VE : Spec T E} {VF : Spec T F} :
+  forall (R : SRelt VE VF) (P : SPrec VE VF),
+  SStable R P ->
+  Stable R (LiftSPrec P).
+unfold SStable, stableSPrec, Stable, stablePrec.
+unfold sub, ssub, subSPrec, subPrec.
+unfold LiftSPrec, LiftSRelt in *.
+intros. psimpl. specialize (H1 x1 eq_refl).
+psimpl. exists x0. split. easy.
+apply H. exists x, x1. easy.
+Qed.
+
+Lemma liftSReltStable {T E F} {VE : Spec T E} {VF : Spec T F} :
+  forall (R : SRelt VE VF) (Q : SRelt VE VF),
+  SStable R Q ->
+  Stable R (LiftSRelt Q).
+unfold SStable, stableSRelt, Stable, stableRelt.
+unfold sub, ssub, subSRelt, subRelt.
+unfold LiftSRelt in *. intros. psimpl.
+specialize (H0 x eq_refl). psimpl.
+specialize (H2 x2 eq_refl). psimpl.
+exists x1. split. easy.
+apply H. exists x0, x2. easy.
+Qed.
+
+Inductive SRTC {T E F} {VE : Spec T E} {VF : Spec T F} (R : SRelt VE VF) : SRelt VE VF :=
+| RTCRefl s ρ : SRTC R s ρ s ρ
+| RTCStep s ρ t σ r τ :
+    R s ρ t σ ->
+    SRTC R t σ r τ ->
+    SRTC R s ρ r τ.
+
+
+Ltac psimpl :=
+repeat lazymatch goal with
+| [ H : prComp ?P ?R ?s ?ρ ?t ?σ |- _ ] => destruct H
+| [ H : ReltCompose ?P ?Q ?s ?ρ ?t ?σ |- _] => destruct H
+| [ H : PrecCompose ?P ?Q ?s ?ρ |- _] => destruct H
+| [ H : SReltCompose ?P ?Q ?s ?ρ ?t ?σ |- _] => destruct H
+| [ H : SPrecCompose ?P ?Q ?s ?ρ |- _] => destruct H
+| [ H : ?P /\ ?Q |- _ ] => destruct H
+| [ H : exists x, ?P |- _ ] => destruct H
+| [ H : ReltToPrec ?R ?s ?ρ |- _ ] => destruct H
+| [ H : PrecToRelt ?R ?s ?ρ ?t ?σ |- _ ] => destruct H
+end;
+simpl in *;
+subst;
+repeat lazymatch goal with
+| [ H : ?A, H' : ?A |- _] => clear H'
+end.
+
+Ltac psplit :=
+match goal with
+| [ |- ReltCompose ?P ?Q ?s ?ρ ?t ?σ ] =>
+    do 2 eexists; split
+| [ |- PrecCompose ?P ?Q ?s ?ρ ] =>
+    do 2 eexists; split
+| [ |- SReltCompose ?P ?Q ?s ?ρ ?t ?σ ] =>
+    do 2 eexists; split
+| [ |- SPrecCompose ?P ?Q ?s ?ρ ] =>
+    do 2 eexists; split
+| [ |- prComp ?P ?Q ?s ?p ?t ?q ] =>
+  split
+| [ |- _ ] => fail "Cannot split on this goal"
+end.
